libs/ffi/mitlsffi.h
@@ -81,6 +81,9 @@ struct _FFI_mitls_callbacks {
 // Connect to a TLS server
 extern int MITLS_CALLCONV FFI_mitls_connect(struct _FFI_mitls_callbacks *callbacks, /* in */ mitls_state *state, /* out */ char **outmsg, /* out */ char **errmsg);
 
+// Resume a previously-established ticket
+extern int MITLS_CALLCONV FFI_mitls_resume(struct _FFI_mitls_callbacks *callbacks, /* in */ mitls_state *state, /* in */ mitls_ticket *ticket, /* out */ char **errmsg);
+
 // Act as a TLS server to a client
 extern int MITLS_CALLCONV FFI_mitls_accept_connected(struct _FFI_mitls_callbacks *callbacks, /* in */ mitls_state *state, /* out */ char **outmsg, /* out */ char **errmsg);
 
